Committed WIP

gf_mul_distr_gen.py
@@ -1,0 +1,30 @@
+# could optimize this to cache for the n's we need and then just call it later
+def construct_tree(n):
+  leaf = "destruct b15. reflexivity. reflexivity. "
+  if n > 15:
+    return ""
+  if n == 15:
+    return leaf
+  current_string = ""
+  for i in range(n,16):
+    current_string += "destruct b"+str(i)+". " 
+  current_string += "reflexivity. reflexivity. "
+  return construct_tree(n+1) + current_string + construct_tree(n+1)
+
+
+
+s = ""
+for i in range(15, -1, -1):
+  # construct a tree with the top node being i-1->15
+  for j in range(i, 16):
+    s+= "destruct b" + str(j)+". "
+    
+  s+=  "reflexivity. reflexivity. "
+  
+  s+=construct_tree(i+1)
+  s+= "\n"
+  
+# print(s)
+with open ("proof_output2.txt", "w") as f:
+    f.write(s)
+
